Proved the safety of merging the first two stages

Kami/Ex/DecExec.v
@@ -1,5 +1,5 @@
 Require Import Kami.
-Require Import Lib.Struct Lib.Indexer.
+Require Import Lib.FinNotations Lib.Struct Lib.Indexer.
 Require Import Ex.ProcMemSpec Ex.PipelinedProc.
 
 Set Implicit Arguments.
@@ -16,7 +16,7 @@ Section DecExec.
 
   Local Notation doMem := (doMem dataK addrSize).
   Local Notation toHost := (toHost dataK).
-  Local Notation D2E := (D2E addrSize rfSize).
+  Local Notation D2E := (D2E addrSize rfSize pgmSize).
   Local Notation sbSearch1 := (sbSearch1 rfSize).
   Local Notation sbSearch2 := (sbSearch2 rfSize).
   Local Notation sbSearch3 := (sbSearch3 rfSize).
@@ -30,7 +30,7 @@ Section DecExec.
       Register "pc" : Bit pgmSize <- pcInit
       with Register "pgm" : Vector instK pgmSize <- pgmInit
 
-      with Rule "deArith" :=
+      with Rule "decexecArith" :=
         Read pc: Bit pgmSize <- "pc";
         Read pgm <- "pgm";
         LET inst <- #pgm@[#pc];
@@ -55,7 +55,7 @@ Section DecExec.
         Write "pc" <- #pc + $1;
         Retv
 
-      with Rule "deLd" :=
+      with Rule "decexecLd" :=
         Read pc: Bit pgmSize <- "pc";
         Read pgm <- "pgm";
         LET inst <- #pgm@[#pc];
@@ -75,7 +75,7 @@ Section DecExec.
         Write "pc" <- #pc + $1;
         Retv
 
-      with Rule "deSt" :=
+      with Rule "decexecSt" :=
         Read pc: Bit pgmSize <- "pc";
         Read pgm <- "pgm";
         LET inst <- #pgm@[#pc];
@@ -94,7 +94,7 @@ Section DecExec.
         Write "pc" <- #pc + $1;
         Retv
 
-      with Rule "deTh" :=
+      with Rule "decexecTh" :=
         Read pc: Bit pgmSize <- "pc";
         Read pgm <- "pgm";
         LET inst <- #pgm@[#pc];
@@ -113,8 +113,8 @@ Section DecExec.
 
   Definition decexecSep :=
     ((decoder dec pcInit pgmInit)
-       ++ (d2e addrSize rfSize)
-       ++ (executer addrSize rfSize exec))%kami.
+       ++ (d2e addrSize rfSize pgmSize)
+       ++ (executer addrSize rfSize pgmSize exec))%kami.
 
   Hint Unfold decexecSep decexec: ModuleDefs.
 
@@ -124,13 +124,6 @@ Section DecExec.
   Qed.
   Hint Resolve decexecSep_ModEquiv.
 
-  Definition decexec_ruleMap (o: RegsT): string -> option string :=
-    "execArith" |-> "deArith";
-      "execLd" |-> "deLd";
-      "execSt" |-> "deSt";
-      "execTh" |-> "deTh"; ||.
-  Hint Unfold decexec_ruleMap: MethDefs.
-
   (* Eval vm_compute in (namesOf (getRegInits decexecSep)). *)
   (* = ["pc"%string; "pgm"%string; "elt.d2e"%string; "full.d2e"%string] *)
   (*   : list string *)
@@ -139,14 +132,33 @@ Section DecExec.
   (*   : list string *)
   Definition decexec_regMap (r: RegsT): RegsT :=
     (mlet pcv : (Bit pgmSize) <- r |> "pc";
-       mlet pgmv : (Vector instK pgmSize) <- r |> "pgm";
-       mlet d2efullv : Bool <- r |> "d2e"--"full";
-       mlet d2eeltv : Struct D2E <- r |> "d2e"--"elt";
-
-       (["pgm" <- existT _ _ pgmv]
-        +["pc" <- existT _ _ (if d2efullv then pcv ^+ $1 else pcv)])%fmap
-    )%mapping.
+     mlet pgmv : (Vector instK pgmSize) <- r |> "pgm";
+     mlet d2efullv : Bool <- r |> "d2e"--"full";
+     mlet d2eeltv : (Struct D2E) <- r |> "d2e"--"elt";
+     (["pgm" <- existT _ _ pgmv]
+      +["pc" <- existT _ (SyntaxKind (Bit pgmSize))
+             (if d2efullv then d2eeltv F7 else pcv)])%fmap)%mapping.
   Hint Unfold decexec_regMap: MapDefs.
+  
+  (* Definition decexec_regMap (ir sr: RegsT): Prop. *)
+  (*   kexistv "pc"%string ipcv ir (Bit pgmSize). *)
+  (*   kexistv "pgm"%string ipgmv ir (Vector instK pgmSize). *)
+  (*   kexistv "d2e"--"full" id2efullv ir Bool. *)
+  (*   kexistv "d2e"--"elt" id2eeltv ir (Struct D2E). *)
+  (*   kexistv "pc"%string spcv sr (Bit pgmSize). *)
+  (*   kexistv "pgm"%string spgmv sr (Vector instK pgmSize). *)
+  (*   refine (_ /\ _). *)
+  (*   - exact (ipgmv = spgmv). *)
+  (*   - exact (ipcv = if id2efullv then spcv ^+ $1 else spcv). *)
+  (* Defined. *)
+  (* Hint Unfold decexec_regMap: MethDefs. *)
+
+  Definition decexec_ruleMap (o: RegsT): string -> option string :=
+    "executeArith" |-> "decexecArith";
+      "executeLd" |-> "decexecLd";
+      "executeSt" |-> "decexecSt";
+      "executeTh" |-> "decexecTh"; ||.
+  Hint Unfold decexec_ruleMap: MethDefs.
 
   Definition decexecSepInl: sigT (fun m: Modules => decexecSep <<== m).
   Proof.
@@ -165,6 +177,78 @@ Section DecExec.
     exact (existT _ _ Him).
   Defined.
 
+  Definition decexec_inv_body
+             (pgmv: fullType type (SyntaxKind (Vector instK pgmSize)))
+             (d2efullv: fullType type (SyntaxKind Bool))
+             (d2eeltv: fullType type (SyntaxKind (Struct D2E))) :=
+    d2efullv = true ->
+    let pc := d2eeltv F7 in
+    let inst := evalExpr (#pgmv@[#pc])%kami_expr in
+    d2eeltv F1 = evalExpr (getOp dec inst) /\
+    d2eeltv F2 = evalExpr (getArithOp dec inst) /\
+    d2eeltv F3 = evalExpr (getSrc1 dec inst) /\
+    d2eeltv F4 = evalExpr (getSrc2 dec inst) /\
+    d2eeltv F5 = evalExpr (getDst dec inst) /\
+    d2eeltv F6 = evalExpr (getAddr dec inst).
+
+  Record decexec_inv (o: RegsT): Prop :=
+    { pcv: fullType type (SyntaxKind (Bit pgmSize));
+      Hpcv: M.find "pc"%string o = Some (existT _ _ pcv);
+      pgmv: fullType type (SyntaxKind (Vector instK pgmSize));
+      Hpgmv: M.find "pgm"%string o = Some (existT _ _ pgmv);
+      d2efullv: fullType type (SyntaxKind Bool);
+      Hd2efullv: M.find "full.d2e"%string o = Some (existT _ _ d2efullv);
+      d2eeltv: fullType type (SyntaxKind (Struct D2E));
+      Hd2eeltv: M.find "elt.d2e"%string o = Some (existT _ _ d2eeltv);
+
+      Hpcinv: d2efullv = true -> pcv = d2eeltv F7 ^+ $1;
+      Hdeinv: decexec_inv_body pgmv d2efullv d2eeltv
+    }.
+  Hint Unfold decexec_inv_body : InvDefs.
+
+  Ltac decexec_inv_tac :=
+    try match goal with
+    | [H: decexec_inv _ |- _] => destruct H
+    end;
+    kinv_red;
+    econstructor; (* let's prove that the invariant holds for the next state *)
+    try (findReify; (reflexivity || eassumption); fail);
+    kinv_red; (* unfolding invariant definitions *)
+    repeat (* cheaper than "intuition" *)
+      (match goal with
+       | [ |- _ /\ _ ] => split
+       end);
+    try eassumption; intros; try reflexivity;
+    intuition kinv_simpl; intuition idtac.
+
+  Lemma decexec_inv_ok':
+    forall init n ll,
+      init = initRegs (getRegInits (projT1 decexecSepInl)) ->
+      Multistep (projT1 decexecSepInl) init n ll ->
+      decexec_inv n.
+  Proof.
+    induction 2.
+    - unfold getRegInits, decexecSepInl, projT1.
+      decexec_inv_tac; simpl in *; kinv_simpl.
+    - kinvert.
+      + mred.
+      + mred.
+      + kinv_dest_custom decexec_inv_tac.
+      + kinv_dest_custom decexec_inv_tac.
+      + kinv_dest_custom decexec_inv_tac.
+      + kinv_dest_custom decexec_inv_tac.
+      + kinv_dest_custom decexec_inv_tac.
+  Qed.
+
+  Lemma decexec_inv_ok:
+    forall o,
+      reachable o (projT1 decexecSepInl) ->
+      decexec_inv o.
+  Proof.
+    intros; inv H; inv H0.
+    eapply decexec_inv_ok'; eauto.
+  Qed.
+  
   Theorem decexec_ok: decexecSep <<== decexec.
   Proof.
     intros.
@@ -178,12 +262,40 @@ Section DecExec.
     (* 3) simulation *)
     (* let invs := (eval hnf in (invariants cfg)) in *)
     (* kinv_add_rep invs; *)
+    kinv_add decexec_inv_ok.
+    kinv_add_end.
     kinvert.
-    (* TODO: add at least the most basic invariant --
-     * the state always has some register values. *)
-    (* - kinv_magic_with idtac idtac. *)
-
-  Admitted.
+    - kinv_action_dest.
+      kinv_custom decexec_inv_tac.
+      + kinv_regmap_red.
+        kinv_constr.
+      + kinv_regmap_red.
+        kinv_constr.
+    - kinv_action_dest.
+      kinv_custom decexec_inv_tac.
+      + kinv_regmap_red.
+        kinv_constr; kinv_eq; kinv_finish.
+      + kinv_regmap_red.
+        kinv_constr; kinv_eq.
+    - kinv_action_dest.
+      kinv_custom decexec_inv_tac.
+      + kinv_regmap_red.
+        kinv_constr; kinv_eq; kinv_finish.
+      + kinv_regmap_red.
+        kinv_constr; kinv_eq.
+    - kinv_action_dest.
+      kinv_custom decexec_inv_tac.
+      + kinv_regmap_red.
+        kinv_constr; kinv_eq; kinv_finish.
+      + kinv_regmap_red.
+        kinv_constr; kinv_eq.
+    - kinv_action_dest.
+      kinv_custom decexec_inv_tac.
+      + kinv_regmap_red.
+        kinv_constr; kinv_eq; kinv_finish.
+      + kinv_regmap_red.
+        kinv_constr; kinv_eq.
+  Qed.
   
 End DecExec.
 
